src/AlgEffectus/Core/TypeSafety.lean
@@ -50,6 +50,38 @@ mutual
     (hh : TyHdl σ Γ h C D) :
     TyHdl σ (Γ.insert x A) h C D := by
     admit
+
+/--
+If `op` is a member of the effect set `Δ` **and** does **not** occur in the
+list of handled operations `ops`, then it is still a member of
+`CTy.eraseMany Δ ops`.  We will use this fact to show that an un‑handled
+operation persists after the erasure passes performed by a handler.
+-/
+lemma mem_eraseMany_of_mem
+    {Δ : Finset OpName} {ops : List OpName} {op : OpName}
+    (hΔ   : op ∈ Δ)
+    (hnot : op ∉ ops) :
+    op ∈ CTy.eraseMany Δ ops := by
+  induction ops with
+  | nil => simpa [CTy.eraseMany] using hΔ
+  | cons hd tl ih =>
+      have hnot_tl : op ∉ tl := by
+        intro h_in; exact hnot (List.mem_cons_of_mem _ h_in)
+      have ih' := ih hnot_tl
+      by_cases hop : op = hd
+      · rw [← hop]
+        simp [CTy.eraseMany] at *
+        exact (False.elim (hnot.left hop))
+      · admit
+        -- have h_mem_in_Δ_erase : op ∈ (Δ.erase hd) := by
+        --   have : op ∈ Δ ∧ op ≠ hd := ⟨hΔ, hop⟩
+        --   simpa [Finset.mem_erase] using this
+        -- have h_rec :
+        --     op ∈ CTy.eraseMany (Δ.erase hd) tl :=
+        --   mem_eraseMany_of_mem h_mem_in_Δ_erase hnot_tl
+        -- -- Now rewrite the goal and finish with `simpa`.
+        -- simpa [CTy.eraseMany, hop] using h_rec
+
 end
 
 mutual
@@ -58,205 +90,237 @@ mutual
     unfold substComp substValue StateT.run
     simp [substCompM]; rfl
 
-  lemma subst_val_preserves
-      {σ Γ x vA A v B}
-      (hv : σ, Γ ⊢ᵥ vA : A)
-      (hvs: σ, (Γ.insert x A) ⊢ᵥ v : B)
-    : σ, Γ ⊢ᵥ (substValue x vA v) : B := by
-    unfold substValue StateT.run
-    cases v with
-    | varV n => cases hvs with
-      | var h_mem =>
-        simp [substValueM] at *
-        split_ifs with hnx
-        · -- 1.  n = x
-          cases hnx
-          have hAB : A = B := by simpa using h_mem
-          cases hAB; simpa using hv
-        · -- 2.  n ≠ x
-          have hΓ : Γ.lookup n = some B := by
-            rw [← h_mem]; simp [hnx]
-          simpa using TyVal.var hΓ
-    | ttV => cases hvs with
-      | tt => simpa [substValueM] using TyVal.tt
-    | ffV => cases hvs with
-      | ff => simpa [substValueM] using TyVal.ff
-    | funV x c => cases hvs with | fun_ hbody =>
-      rename_i x' A' C
-      simp [substValueM] at *
-      split_ifs with hnx hxf
-      · -- 1.  x = x'
-        cases hnx
-        split; rename_i  y result' snd' heq'
-        cases heq'
-        apply TyVal.fun_; simp at hbody; exact hbody
-      · -- 2.  x ≠ x' ∧ x ∈ freeVarsValue vA
-        apply TyVal.fun_
-        simp [substCompM]
-        cases hbody
-        repeat sorry
-      · -- 3. x ≠ x' ∧ x ∉ freeVarsValue vA
-        apply TyVal.fun_
-        simp [substCompM]
-        cases hbody
-        repeat sorry
-    | handV h =>
-      simp [substValueM] at *
-      cases h with
-      | mk rb rc opcls =>
-        cases hvs
-        rename_i C D th
-        simp [substValueM] at *
-        split_ifs with hrbx
-        · admit
-        · admit
+  lemma subst_valM_preserves
+    {σ Γ x vA A v B ctx}
+    (hv : σ, Γ ⊢ᵥ vA : A)
+    (hvs: σ, (Γ.insert x A) ⊢ᵥ v : B)
+    : σ, Γ ⊢ᵥ (substValueM x vA v ctx).1 : B := by
+  -- unfold substValue StateT.run
+  -- cases v with
+  -- | varV n => cases hvs with
+  --   | var h_mem =>
+  --     simp [substValueM] at *
+  --     split_ifs with hnx
+  --     · -- 1.  n = x
+  --       cases hnx
+  --       have hAB : A = B := by simpa using h_mem
+  --       cases hAB; simpa using hv
+  --     · -- 2.  n ≠ x
+  --       have hΓ : Γ.lookup n = some B := by
+  --         rw [← h_mem]; simp [hnx]
+  --       simpa using TyVal.var hΓ
+  -- | ttV => cases hvs with
+  --   | tt => simpa [substValueM] using TyVal.tt
+  -- | ffV => cases hvs with
+  --   | ff => simpa [substValueM] using TyVal.ff
+  -- | funV x c => cases hvs with | fun_ hbody =>
+  --   rename_i x' A' C
+  --   simp [substValueM] at *
+  --   split_ifs with hnx hxf
+  --   · -- 1.  x = x'
+  --     cases hnx
+  --     split; rename_i  y result' snd' heq'
+  --     cases heq'
+  --     apply TyVal.fun_; simp at hbody; exact hbody
+  --   · -- 2.  x ≠ x' ∧ x ∈ freeVarsValue vA
+  --     apply TyVal.fun_
+  --     simp [substCompM]
+  --     cases hbody
+  --     repeat sorry
+  --   · -- 3. x ≠ x' ∧ x ∉ freeVarsValue vA
+  --     apply TyVal.fun_
+  --     simp [substCompM]
+  --     cases hbody
+  --     repeat sorry
+  -- | handV h =>
+  --   simp [substValueM] at *
+  --   cases h with
+  --   | mk rb rc opcls =>
+  --     cases hvs
+  --     rename_i C D th
+  --     simp [substValueM] at *
+  --     split_ifs with hrbx
+  --     · admit
+  --     · admit
 
-lemma subst_valM_preserves
-  {σ Γ x vA A v B ctx}
-  (hv : σ, Γ ⊢ᵥ vA : A)
-  (hvs: σ, (Γ.insert x A) ⊢ᵥ v : B)
-  : σ, Γ ⊢ᵥ (substValueM x vA v ctx).1 : B := by
-  admit
+    admit
 
-lemma subst_compM_preserves
-  {σ Γ x vA A c C ctx}
-  (hv : σ, Γ ⊢ᵥ vA : A)
-  (hc : σ, (Γ.insert x A) ⊢ c : C) :
-  σ, Γ ⊢ (substCompM x vA c ctx).1 : C := by
-  revert ctx
-  cases c with
-  | retC v =>
-    intro ctx
-    cases hc with | ret hv_v =>
-    rename_i B Δ
-    simp [substCompM]
-    apply TyComp.ret
-    apply subst_valM_preserves hv hv_v
-
-  | callC op arg k body =>
-    intro ctx
-    cases hc with | call_ hfresh sig targ tcont mem =>
-    rename_i Aᵢ Bᵢ A' Δ
-    simp [substCompM]
-    split_ifs with hkx
-    · -- 1. k = x
-      cases hkx; simp at hfresh
-    · -- 2. k ≠ x
-      have h₁ : σ, Γ ⊢ᵥ (substValueM x vA arg ctx).1 : Aᵢ := by apply subst_valM_preserves hv targ
-      have hfresh': Γ.lookup k = none := by
-        simpa [hkx] using hfresh
-      have hv' : σ, Γ.insert k Bᵢ ⊢ᵥ vA : A := by
-        exact weaken_val (Or.inl hfresh') hv
-      have tcont' : σ, (Γ.insert k Bᵢ).insert x A ⊢ body : A' !{Δ} := by
-        rw [CtxLemmas.insert_insert_of_ne hkx]; exact tcont
-      have hbody' : σ, Γ.insert k Bᵢ ⊢
-      (substCompM x vA body (substValueM x vA arg ctx).2).1 : A' !{Δ} := by
-        exact subst_compM_preserves hv' tcont'
-      exact TyComp.call_ hfresh' sig h₁ hbody' mem
-  | seqC x c₁ c₂ => admit
-  | ifC b t e => admit
-  | appC f a => admit
-  | withC h c => admit
-
-  lemma subst_comp_preserves
-      {σ Γ x vA A c C}
-      (hv : σ, Γ ⊢ᵥ vA : A)
-      (hc : σ, (Γ.insert x A) ⊢ c : C)
-    : σ, Γ ⊢ (substComp x vA c) : C := by
+  lemma subst_compM_preserves
+    {σ Γ x vA A c C ctx}
+    (hv : σ, Γ ⊢ᵥ vA : A)
+    (hc : σ, (Γ.insert x A) ⊢ c : C) :
+    σ, Γ ⊢ (substCompM x vA c ctx).1 : C := by
+    revert ctx
     cases c with
     | retC v =>
+      intro ctx
       cases hc with | ret hv_v =>
       rename_i B Δ
-      simp [substComp]
+      simp [substCompM]
       apply TyComp.ret
-      apply subst_val_preserves hv hv_v
+      apply subst_valM_preserves hv hv_v
+
     | callC op arg k body =>
+      intro ctx
       cases hc with | call_ hfresh sig targ tcont mem =>
       rename_i Aᵢ Bᵢ A' Δ
-      simp [substComp]
+      simp [substCompM]
       split_ifs with hkx
       · -- 1. k = x
         cases hkx; simp at hfresh
       · -- 2. k ≠ x
-        have h₁ : σ, Γ ⊢ᵥ (substValue x vA arg) : Aᵢ := by apply subst_val_preserves hv targ
+        have h₁ : σ, Γ ⊢ᵥ (substValueM x vA arg ctx).1 : Aᵢ := by apply subst_valM_preserves hv targ
         have hfresh': Γ.lookup k = none := by
           simpa [hkx] using hfresh
-        apply TyComp.call_ hfresh' sig h₁
-        · simp [StateT.run]
-          apply weaken_comp (Or.inl hfresh')
-          · admit
-        · exact mem
+        have hv' : σ, Γ.insert k Bᵢ ⊢ᵥ vA : A := by
+          exact weaken_val (Or.inl hfresh') hv
+        have tcont' : σ, (Γ.insert k Bᵢ).insert x A ⊢ body : A' !{Δ} := by
+          rw [CtxLemmas.insert_insert_of_ne hkx]; exact tcont
+        have hbody' : σ, Γ.insert k Bᵢ ⊢
+        (substCompM x vA body (substValueM x vA arg ctx).2).1 : A' !{Δ} := by
+          exact subst_compM_preserves hv' tcont'
+        exact TyComp.call_ hfresh' sig h₁ hbody' mem
     | seqC x c₁ c₂ => admit
     | ifC b t e => admit
     | appC f a => admit
     | withC h c => admit
 
-  lemma subst_hdl_preserves
+  lemma subst_hdlM_preserves
       {σ Γ x vA A h C D}
       (hv : σ, Γ ⊢ᵥ vA : A)
       (hh : TyHdl σ (Γ.insert x A) h C D)
-    : TyHdl σ Γ (substHandler x vA h) C D
-    := by admit
+    : TyHdl σ Γ (substHandler x vA h) C D := by
+    admit
 end
+
+lemma subst_val_preserves
+    {σ Γ x vA A v B}
+    (hv : σ, Γ ⊢ᵥ vA : A)
+    (hvs: σ, (Γ.insert x A) ⊢ᵥ v : B)
+  : σ, Γ ⊢ᵥ (substValue x vA v) : B := by
+  exact subst_valM_preserves hv hvs
+lemma subst_comp_preserves
+    {σ Γ x vA A c C}
+    (hv : σ, Γ ⊢ᵥ vA : A)
+    (hc : σ, (Γ.insert x A) ⊢ c : C)
+  : σ, Γ ⊢ (substComp x vA c) : C := by
+  exact subst_compM_preserves hv hc
+
+lemma subst_hdl_preserves
+    {σ Γ x vA A h C D}
+    (hv : σ, Γ ⊢ᵥ vA : A)
+    (hh : TyHdl σ (Γ.insert x A) h C D)
+  : TyHdl σ Γ (substHandler x vA h) C D := by
+  exact subst_hdlM_preserves hv hh
 
 theorem preservation {σ Γ c c' C}
   (hTy: σ, Γ ⊢ c : C)
   (hStep: c ⤳ c')
-: σ, Γ ⊢ c' : C
-:= by
+: σ, Γ ⊢ c' : C := by
   induction hStep generalizing C with
   | seq_step h₁ ih  =>
-    rename_i x c₁ c₁' c₂
+    rename_i x _ c₁' c₂
     cases hTy with | seq t₁ t₂ =>
-      rename_i A B Δ
-      have hTy₁' : σ, Γ ⊢ c₁' : (A !{Δ}) := by
-        apply ih; exact t₁
-      have hTy₂' : σ, Γ.insert x A ⊢ c₂ : (B !{Δ}) := by
-        exact t₂
-      apply TyComp.seq hTy₁' hTy₂'
+    rename_i A B Δ
+    have hTy₁' : σ, Γ ⊢ c₁' : (A !{Δ}) := by apply ih; exact t₁
+    have hTy₂' : σ, Γ.insert x A ⊢ c₂ : (B !{Δ}) := by exact t₂
+    apply TyComp.seq hTy₁' hTy₂'
   | seq_return =>
-    rename_i x v c₁
     cases hTy with | seq t₁ t₂ =>
-      rename_i A B Δ
-      cases t₁ with | ret t₁' =>
-        exact subst_comp_preserves t₁' t₂
+    cases t₁ with | ret t₁' =>
+    exact subst_comp_preserves t₁' t₂
   | seq_op     =>
-    rename_i op x v y c₁ c₂ hxy
+    rename_i _ x _ y c₁ c₂ hxy
     cases hTy with | seq t₁ t₂ =>
-      rename_i A B Δ
-      cases t₁ with | call_ hfresh sig targ tcont mem =>
-      rename_i Aᵢ Bᵢ
-      have tcont' : σ, Γ.insert y Bᵢ ⊢ Computation.seqC x c₁ c₂ : B !{Δ} := by
-        apply TyComp.seq tcont
-        have hyx : y ≠ x := Ne.symm hxy
-        rw [CtxLemmas.insert_insert_of_ne hyx]
-        apply weaken_comp
-        · rw [CtxLemmas.lookup_insert_ne hyx]; rw [hfresh]; simp
-        · exact t₂
-      exact TyComp.call_ hfresh sig targ tcont' mem
-  | if_true  =>
-    rename_i c₁' c₂'
-    cases hTy with | if_ tb tt te => exact tt
-  | if_false   =>
-    rename_i c₁' c₂'
-    cases hTy with | if_ tb tt te => exact te
+    rename_i _ B Δ
+    cases t₁ with | call_ hfresh sig targ tcont mem =>
+    rename_i _ Bᵢ
+    have tcont' : σ, Γ.insert y Bᵢ ⊢ Computation.seqC x c₁ c₂ : B !{Δ} := by
+      apply TyComp.seq tcont
+      have hyx : y ≠ x := Ne.symm hxy
+      rw [CtxLemmas.insert_insert_of_ne hyx]
+      apply weaken_comp
+      · rw [CtxLemmas.lookup_insert_ne hyx]; rw [hfresh]; simp
+      · exact t₂
+    exact TyComp.call_ hfresh sig targ tcont' mem
+  | if_true    => cases hTy with | if_ tb tt te => exact tt
+  | if_false   => cases hTy with | if_ tb tt te => exact te
   | app_β      =>
-    rename_i x c₁' v
     cases hTy with | app tf ta =>
-      apply subst_comp_preserves ta
-      cases tf with | fun_ hbody => exact hbody
+    apply subst_comp_preserves ta
+    cases tf with | fun_ hbody => exact hbody
   | with_step hStep ih =>
-    rename_i h c₁' c₂'
     cases hTy with | with_ th tc =>
-      rename_i C'
-      apply TyComp.with_ th; exact ih tc
+    apply TyComp.with_ th; exact ih tc
   | with_ret hyRet  =>
-    rename_i h c₁
     cases hTy with | with_ th tc =>
-      rename_i x c_ret C'
-      admit
-  | with_handled hySucc => admit
-  | with_unhandled => admit
+    cases tc with | ret hv_c₁ =>
+    cases th with | hand hh =>
+    cases hh with | mk _ rest _ _ =>
+    simp [Handler.getRetClause] at hyRet
+    rw [← hyRet.right]; rw [hyRet.left] at rest
+    unfold substComp StateT.run
+    exact subst_compM_preserves hv_c₁ rest
+  | with_handled hySucc =>
+    rename_i h opName v x y k cᵢ cBody
+    cases hTy with | with_ th tc =>
+    rename_i CParam
+    cases th with | hand hh =>
+    cases tc with | call_ hfresh sig targ tcont mem =>
+    rename_i Aᵢ Bᵢ A' Δ
+    cases hh with | mk hkfresh ret hops heff =>
+    rename_i rb rc opcs B Δ'
+    simp [Handler.findOpClause] at hySucc
+    have hh : TyHdl σ Γ (Handler.mk rb rc opcs) (A' !{Δ}) (B !{Δ'}) := by
+      exact TyHdl.mk hkfresh ret hops heff
+    have th₀ : σ, Γ ⊢ᵥ Value.handV (Handler.mk rb rc opcs) : VTy.hdlT (A' !{Δ}) (B !{Δ'}) :=
+      TyVal.hand hh
+    rcases hySucc with ⟨currOp, h_eq⟩
+    unfold substComp StateT.run
+    have th₁ : σ, Γ.insert y Bᵢ ⊢ᵥ Value.handV (Handler.mk rb rc opcs)
+        : VTy.hdlT (A' !{Δ}) (B !{Δ'}) := by
+      exact weaken_val (Or.inl hfresh) th₀
+    have th₂ : σ, Γ.insert k (Bᵢ.funT (B !{Δ'})) ⊢ᵥ v : Aᵢ := by
+      apply weaken_val; apply Or.inl; exact (hkfresh (List.mem_of_find?_eq_some h_eq)).1; exact targ
+    have h_x_neq_k : x ≠ k := (hkfresh (List.mem_of_find?_eq_some h_eq)).2
+    have th₃ : σ, (Γ.insert k (Bᵢ.funT (B !{Δ'}))).insert x Aᵢ ⊢ cᵢ : B !{Δ'} := by admit
+      -- have h_hops := hops (List.mem_of_find?_eq_some h_eq) sig
+      -- rw [Finmap.insert_comm x Aᵢ k (Bᵢ.funT (B !{Δ'})) h_x_neq_k]
+      -- exact h_hops
+    exact subst_compM_preserves (TyVal.fun_ (TyComp.with_ (TyVal.hand (weaken_hdl (Or.inl hfresh) hh)) tcont))
+      (subst_comp_preserves th₂ th₃)
+  | with_unhandled hyFail =>
+    rename_i h opName v y cBody
+    cases hTy with | with_ th tc =>
+    rename_i CParam
+    cases th with | hand hh =>
+    cases tc with | call_ hfresh sig targ tcont mem =>
+    rename_i Aᵢ Bᵢ A' Δ
+    cases hh with | mk hkfresh ret hops heff =>
+    rename_i rb rc opcs B Δ'
+    simp [Handler.findOpClause] at hyFail
+    have hh : TyHdl σ Γ (Handler.mk rb rc opcs) (A' !{Δ}) (B !{Δ'}) := by
+      exact TyHdl.mk hkfresh ret hops heff
+    have th₀ : σ, Γ ⊢ᵥ Value.handV (Handler.mk rb rc opcs)
+        : VTy.hdlT (A' !{Δ}) (B !{Δ'}) := TyVal.hand hh
+    have th' : σ, Γ.insert y Bᵢ ⊢ᵥ Value.handV (Handler.mk rb rc opcs)
+        : VTy.hdlT (A' !{Δ}) (B !{Δ'}) :=
+      weaken_val (Or.inl hfresh) th₀
+    have tcont' : σ, Γ.insert y Bᵢ ⊢
+        Computation.withC (Value.handV (Handler.mk rb rc opcs)) cBody
+        : B !{Δ'} := by
+      exact TyComp.with_ th' tcont
+    have mem' : opName ∈ Δ' := by
+      have hnot : opName ∉ List.map (fun t => t.1) opcs := by
+        intro h_in
+        rcases List.mem_map.1 h_in with
+          ⟨⟨op' , x' , k' , body'⟩, h_mem, h_eq⟩
+        have hneq := hyFail op' x' k' body' h_mem
+        exact (hneq (by simpa [h_eq]))
+      have hmemErase : opName ∈ CTy.eraseMany Δ (List.map (fun t => t.1) opcs) :=
+        mem_eraseMany_of_mem mem hnot
+      exact heff hmemErase
+    exact TyComp.call_ hfresh sig targ tcont' mem'
 
 theorem progress {σ c A Δ} :
   (σ, ∅ ⊢ c : (A !{Δ})) →
@@ -272,41 +336,3 @@ theorem progress {σ c A Δ} :
   | app tf ta       => admit
   | if_ tb tt te    => admit
   | with_ th tc     => admit
-
--- mutual
---   lemma weaken_val {σ Γ x A v B} (hv : σ, Γ ⊢ᵥ v : B) :
---     σ, (Γ.insert x A) ⊢ᵥ v : B := by
---     cases hv with
---     | var h_mem =>
---       rename_i n; apply TyVal.var
---       simp [Std.HashMap.getElem?_insert]
---       simp at h_mem
---       by_cases h_eq_keys : x = n
---       · rw [← h_eq_keys] at h_mem
---         sorry
---       · split <;> simp_all
---     | tt => exact TyVal.tt
---     | ff => exact TyVal.ff
---     | fun_ hbody =>
---       rename_i x' A' C body; apply TyVal.fun_
---       by_cases h_eq_keys : x = x'
---       · sorry
---       · sorry
---       rw [hΓ]; apply weaken_comp; exact hbody
---     | hand h =>
---       admit
---
---
---   lemma weaken_comp
---       {σ Γ x A c C}
---       (hc : TyComp σ Γ c C) :
---       TyComp σ (Γ.insert x A) c C := by admit
---
---   lemma weaken_hdl {σ Γ x A h C D} (hh : TyHdl σ Γ h C D) :
---     TyHdl σ (Γ.insert x A) h C D := by
---     cases hh with
---     | mk hret hops heff =>
---       rename_i rb rc opcs A' B' Δ Δ'
---       apply TyHdl.mk
---       repeat admit
--- end
